IMPminus_TM/TM_GOTO/TM_to_GOTO_on_List.thy
@@ -1,5 +1,6 @@
 theory TM_to_GOTO_on_List
-  imports GOTO_on_List "IMPminus_TM-Def.Global_Defs" Cook_Levin.Basics
+  imports GOTO_on_List "IMPminus_TM-Def.Global_Defs" Cook_Levin.Basics "List-Index.List_Index"
+          List_Extra
 begin
 
 locale TM_to_GOTO_on_List =
@@ -25,33 +26,34 @@ fun tape_content_to_list :: "(nat \<Rightarrow> symbol) \<Rightarrow> nat \<Righ
   "tape_content_to_list tp 0 = []" |
   "tape_content_to_list tp (Suc n) = (tape_content_to_list tp n) @ [tp n]"
 
-fun s\<^sub>0 :: state\<^sub>l where          
-  "s\<^sub>0 (TP n) = tape_content_to_list (TPS ::: n) MAX_LEN" |
-  "s\<^sub>0 ST = [0]" |
-  "s\<^sub>0 (HP n) = [TPS :#: n]" |
-  "s\<^sub>0 (TMP n) = []"
+fun config_to_state :: "config \<Rightarrow> state\<^sub>l" where
+  "config_to_state (q, tps) (TP n) = tape_content_to_list (tps ::: n) MAX_LEN" |
+  "config_to_state (q, tps) ST = [q]" |
+  "config_to_state (q, tps) (HP n) = [tps :#: n]" |
+  "config_to_state (q, tps) (TMP n) = []"
 
-subsection \<open>Definition of the transform function\<close>
+abbreviation q_chs_enum_list :: "(state \<times> symbol list) list" where
+  "q_chs_enum_list \<equiv> List.product [0..<Q] (product_lists (replicate MAX_LEN [0..<G]))"
 
-value "List.product [0..<5] (product_lists (replicate 4 [0..1]))"
+lemma q_chs_enum_list_distinct: "distinct q_chs_enum_list"
+proof -
+  have "distinct [0..<G]"
+    by simp
+  then have "\<forall>xs \<in> set (replicate MAX_LEN [0..<G]). distinct xs"
+    by fastforce
+  then have "distinct (product_lists (replicate MAX_LEN [0..<G]))"
+    using distinct_product_lists by blast
+  moreover
+  have "distinct [0..<Q]"
+    by fastforce
+  ultimately
+  show ?thesis
+    using distinct_product by blast
+qed
 
-fun entrance_block_gen :: "(state \<times> symbol list) list \<Rightarrow> nat \<Rightarrow> GOTO\<^sub>l_prog" where
-  "entrance_block_gen [] _ = [
-     IF ST = L [Q] THEN GOTO\<^sub>l pc_halt,
-     TMP 0 ::=\<^sub>l ReadChs [0..<K]]" |
-  "entrance_block_gen ((q, chs) # q_chs_s) idx =
-    entrance_block_gen q_chs_s (Suc idx) @ [
-    IF ST = L [q] AND TMP 0 = L chs
-    THEN GOTO\<^sub>l ((Suc (Suc (Q * G ^ MAX_LEN))) + idx * (Suc (3 * K)))]"
+abbreviation q_chs_num :: nat where "q_chs_num \<equiv> Q * G ^ MAX_LEN"
 
-lemma entrance_block_gen_length: "length (entrance_block_gen q_xs_s n) = Suc (Suc (length q_xs_s))"
-  by (induction q_xs_s arbitrary: n) auto
-
-definition entrance_block :: "GOTO\<^sub>l_prog" where
-  "entrance_block =
-   entrance_block_gen (List.product [0..<Q] (product_lists (replicate MAX_LEN [0..<G]))) 0"
-
-lemma entrance_block_length: "length entrance_block = Suc (Suc (Q * G ^ MAX_LEN))"
+lemma q_chs_enum_list_length: "length q_chs_enum_list = q_chs_num"
 proof -
   have "length [0..<G] = G"
     by simp
@@ -66,20 +68,76 @@ proof -
   have "foldr (*) (replicate MAX_LEN G) 1 = fold (*) (replicate MAX_LEN G) 1"
     by force
   ultimately
-  have "length (product_lists (replicate MAX_LEN [0..<G])) = G ^ MAX_LEN"
+  show ?thesis
     using length_product_lists [of "replicate MAX_LEN [0..<G]"]
     by simp
-  then have "length (List.product [0..<Q] (product_lists (replicate MAX_LEN [0..<G]))) =
-             Q * G ^ MAX_LEN"
-    by auto
-  then show ?thesis
-    unfolding entrance_block_def
-    using entrance_block_gen_length
+qed
+
+abbreviation s\<^sub>0 :: state\<^sub>l where "s\<^sub>0 \<equiv> config_to_state (0, TPS)"
+
+subsection \<open>Definition of the transform function\<close>
+
+abbreviation entrance_block_len :: nat where
+  "entrance_block_len \<equiv> Suc (Suc q_chs_num)"
+abbreviation block_for_q_chs_len :: nat where
+  "block_for_q_chs_len \<equiv> Suc (3 * K)"
+
+fun label_of_block_for_q_chs :: "state \<times> symbol list \<Rightarrow> label" where
+  "label_of_block_for_q_chs (q, chs) =
+   Suc entrance_block_len + block_for_q_chs_len * (index q_chs_enum_list (q, chs))"
+
+abbreviation entrance_block :: "GOTO\<^sub>l_prog" where
+  "entrance_block \<equiv> [
+     IF ST = L [Q] THEN GOTO\<^sub>l pc_halt,
+     TMP 0 ::=\<^sub>l ReadChs [0..<K]] @
+     map (\<lambda>(q, chs).
+       IF ST = L [q] AND TMP 0 = L chs
+       THEN GOTO\<^sub>l label_of_block_for_q_chs (q, chs))
+     q_chs_enum_list"
+
+lemma entrance_block_length: "length entrance_block = entrance_block_len"
+  using q_chs_enum_list_length by fastforce
+
+lemma entrance_block_distinct: "distinct entrance_block"
+proof -
+  let ?f = "\<lambda>(q, chs).
+    IF ST = L [q] AND TMP 0 = L chs THEN GOTO\<^sub>l label_of_block_for_q_chs (q, chs)"
+  have "\<forall>q_chs \<in> set q_chs_enum_list. \<forall>q_chs' \<in> set q_chs_enum_list.
+        ?f q_chs = ?f q_chs' \<longrightarrow> q_chs = q_chs'"
+    by fast
+  then have "inj_on ?f (set q_chs_enum_list)"
+    using inj_on_def by fast
+  with q_chs_enum_list_distinct have "distinct (map ?f q_chs_enum_list)"
+    using distinct_map by blast
+  then show "distinct entrance_block"
     by fastforce
 qed
 
-fun block_for_q_and_chs :: "state \<times> action list \<Rightarrow> GOTO\<^sub>l_prog" where
-  "block_for_q_and_chs q_act_s =
+lemma q_chs_in_entrance_block_iff:
+  "(q, chs) \<in> set q_chs_enum_list \<longleftrightarrow>
+   (IF ST = L [q] AND TMP 0 = L chs THEN GOTO\<^sub>l label_of_block_for_q_chs (q, chs))
+    \<in> set (entrance_block)"
+proof
+  let ?f = "\<lambda>(q, chs).
+    IF ST = L [q] AND TMP 0 = L chs THEN GOTO\<^sub>l label_of_block_for_q_chs (q, chs)"
+  fix q chs assume "(q, chs) \<in> set q_chs_enum_list"
+  then have "?f (q, chs) \<in> set (map ?f q_chs_enum_list)" by fastforce
+  then show "(IF ST = L [q] AND TMP 0 = L chs THEN GOTO\<^sub>l label_of_block_for_q_chs (q, chs))
+             \<in> set entrance_block"
+    by force
+next
+  let ?f = "\<lambda>(q, chs).
+    IF ST = L [q] AND TMP 0 = L chs THEN GOTO\<^sub>l label_of_block_for_q_chs (q, chs)"
+  fix q chs
+  assume "(IF ST = L [q] AND TMP 0 = L chs THEN GOTO\<^sub>l label_of_block_for_q_chs (q, chs))
+          \<in> set entrance_block"
+  then have "?f (q, chs) \<in> set entrance_block" by fast
+  then have "?f (q, chs) \<in> set (map ?f q_chs_enum_list)" by force
+  then show "(q, chs) \<in> set q_chs_enum_list" by force
+qed
+
+fun block_for_q_chs :: "state \<times> action list \<Rightarrow> GOTO\<^sub>l_prog" where
+  "block_for_q_chs q_act_s =
      (ST ::=\<^sub>l L [[*] q_act_s]) # \<comment> \<open>update state\<close>
      (concat (map (\<lambda>n. [
         TapeModify n (q_act_s [.] n), \<comment> \<open>tape modification\<close>
@@ -88,7 +146,7 @@ fun block_for_q_and_chs :: "state \<times> action list \<Rightarrow> GOTO\<^sub>
         GOTO\<^sub>l pc_start])
       [0..<K]))" \<comment> \<open>for each tape\<close>
 
-lemma length_block_for_q_and_chs: "length (block_for_q_and_chs q_act_s) = Suc (3 * K)"
+lemma block_for_q_and_chs_length: "length (block_for_q_chs q_act_s) = block_for_q_chs_len"
 proof -
   let ?f = "(\<lambda>n. [
     TapeModify n (q_act_s [.] n), \<comment> \<open>tape modification\<close>
@@ -96,30 +154,202 @@ proof -
       Left \<Rightarrow> MoveLeft n | Right \<Rightarrow> MoveRight n | Stay \<Rightarrow> NOP\<^sub>l, \<comment> \<open>head movement\<close>
     GOTO\<^sub>l pc_start])"
   have "length (?f n) = 3" for n by auto
-  then have "map length (map ?f [0..<K]) = replicate K 3"
-    by (simp add: comp_def map_replicate_trivial)
-  moreover
-  have "sum_list (replicate K 3) = 3 * K"
-    by (simp add: sum_list_replicate)
-  ultimately
-  have "length (concat (map ?f [0..<K])) = 3 * K"
-    by (simp add: length_concat)
+  then have "\<forall>xs \<in> set (map ?f [0..<K]). length xs = 3"
+    by simp
+  then have "length (concat (map ?f [0..<K])) = 3 * K"
+    using length_concat_same_length [where ?xss = "map ?f [0..<K]"]
+    by auto
   then show ?thesis by auto
 qed
 
-definition blocks_for_actions :: "GOTO\<^sub>l_prog" where
-  "blocks_for_actions =
-   concat (map (\<lambda>(q, chs). block_for_q_and_chs ((M!q) chs))
-               (List.product [0..<Q] (product_lists (replicate MAX_LEN [0..<G]))))"
+abbreviation blocks_for_actions :: "GOTO\<^sub>l_prog" where
+  "blocks_for_actions \<equiv>
+   concat (map (\<lambda>(q, chs). block_for_q_chs ((M!q) chs)) q_chs_enum_list)"
 
+lemma blocks_for_actions_length: "length blocks_for_actions = block_for_q_chs_len * q_chs_num"
+proof -
+  let ?f = "\<lambda>(q, chs). block_for_q_chs ((M!q) chs)"  
+  from block_for_q_and_chs_length
+  have "\<forall>q_chs \<in> set q_chs_enum_list. length (?f q_chs) = block_for_q_chs_len" by fast
+  then have "\<forall>blk \<in> set (map ?f q_chs_enum_list). length blk = block_for_q_chs_len" by simp
+  then have "length blocks_for_actions = block_for_q_chs_len * (length q_chs_enum_list)"
+    using length_concat_same_length [where ?xss = "map ?f q_chs_enum_list"]
+    by fastforce
+  then show ?thesis
+    using q_chs_enum_list_length by presburger
+qed
 
-definition GOTO_on_List_Prog :: "GOTO\<^sub>l_prog" where
-  "GOTO_on_List_Prog = HALT\<^sub>l # entrance_block @ blocks_for_actions @ [HALT\<^sub>l]"
+abbreviation GOTO_on_List_Prog :: "GOTO\<^sub>l_prog" where
+  "GOTO_on_List_Prog \<equiv> HALT\<^sub>l # entrance_block @ blocks_for_actions @ [HALT\<^sub>l]"
+
+lemma label_of_block_for_q_chs_correct:
+  assumes "(q, chs) \<in> set q_chs_enum_list"
+  shows "take block_for_q_chs_len (drop (label_of_block_for_q_chs (q, chs)) GOTO_on_List_Prog) =
+         block_for_q_chs ((M!q) chs)"
+proof -
+  let ?idx = "index q_chs_enum_list (q, chs)"
+  let ?f = "\<lambda>(q, chs). block_for_q_chs ((M!q) chs)"
+  let ?q_chs_s_after_q_chs = "drop ?idx q_chs_enum_list"
+  let ?blks_after_label = "drop (block_for_q_chs_len * ?idx) blocks_for_actions"
+
+  from assms have idx_q_chs_lt: "?idx < length q_chs_enum_list"
+    by fastforce
+  then have "hd ?q_chs_s_after_q_chs = q_chs_enum_list ! ?idx"
+    using hd_drop_conv_nth by blast
+  with assms have "hd ?q_chs_s_after_q_chs = (q, chs)"
+    using nth_index by metis
+
+  from idx_q_chs_lt have "?q_chs_s_after_q_chs \<noteq> []"
+    using assms q_chs_enum_list_length
+    by (metis drop_eq_Nil leD)
+
+  from idx_q_chs_lt have label_part_2_not_exceed_prog:
+    "block_for_q_chs_len * ?idx < length blocks_for_actions"
+    using assms blocks_for_actions_length q_chs_enum_list_length
+    using Suc_mult_less_cancel1 by presburger
+  
+  have label_part_1_get_over_entrance_block:
+    "drop (Suc entrance_block_len) GOTO_on_List_Prog = blocks_for_actions @ [HALT\<^sub>l]"
+    using drop_append [where ?xs = "HALT\<^sub>l # entrance_block"
+                         and ?ys = "blocks_for_actions @ [HALT\<^sub>l]"
+                         and ?n = "Suc entrance_block_len"]
+    using entrance_block_length
+    by auto
+
+  from block_for_q_and_chs_length
+  have "\<forall>q_chs \<in> set q_chs_enum_list. length (?f q_chs) = block_for_q_chs_len"
+    by fast
+  then have same_length: "\<forall>xs \<in> set (map ?f q_chs_enum_list). length xs = block_for_q_chs_len"
+    by fastforce
+  with drop_concat_same_length [where ?xss = "map ?f q_chs_enum_list"
+                                  and ?n = "?idx"
+                                  and ?len = block_for_q_chs_len]
+  have "?blks_after_label = concat (drop ?idx (map ?f q_chs_enum_list))"
+    by blast
+  moreover
+  have map_in_out:
+    "drop ?idx (map ?f q_chs_enum_list) = map ?f ?q_chs_s_after_q_chs"
+    using drop_map by fast
+  then have "concat (drop ?idx (map ?f q_chs_enum_list)) =
+             concat (map ?f ?q_chs_s_after_q_chs)"
+    by presburger
+  ultimately
+  have "?blks_after_label = concat (map ?f ?q_chs_s_after_q_chs)"
+    by (simp add: mult.commute)
+  
+  have "length ?blks_after_label \<ge> block_for_q_chs_len"
+  proof -
+    from same_length have "\<forall>xs \<in> set (map ?f ?q_chs_s_after_q_chs). length xs = block_for_q_chs_len"
+      by (metis in_set_dropD map_in_out)
+    then have "length (concat (map ?f ?q_chs_s_after_q_chs)) =
+               block_for_q_chs_len * length ?q_chs_s_after_q_chs"
+      using length_concat_same_length [where ?xss = "map ?f ?q_chs_s_after_q_chs"
+                                         and ?len = block_for_q_chs_len]
+      by (metis length_map)
+    moreover
+    from \<open>?q_chs_s_after_q_chs \<noteq> []\<close> have "length ?q_chs_s_after_q_chs \<ge> 1" by fastforce
+    ultimately
+    have "length (concat (map ?f ?q_chs_s_after_q_chs)) \<ge> block_for_q_chs_len"
+      by (metis mult_le_mono2 nat_mult_1_right)
+    with \<open>?blks_after_label = concat (map ?f ?q_chs_s_after_q_chs)\<close>
+    show ?thesis by argo
+  qed
+
+  from take_concat_same_length [where ?len = block_for_q_chs_len and ?n = 1
+                                  and ?xss = "map ?f ?q_chs_s_after_q_chs"]
+  have "take block_for_q_chs_len (concat (map ?f ?q_chs_s_after_q_chs)) =
+        concat (take 1 (map ?f ?q_chs_s_after_q_chs))"
+    using same_length map_in_out
+    by (metis in_set_dropD nat_mult_1_right)
+  also have "... = hd (map ?f ?q_chs_s_after_q_chs)"
+    using concat_take_1_is_hd \<open>?q_chs_s_after_q_chs \<noteq> []\<close>
+    by blast
+  also have "... = ?f (hd ?q_chs_s_after_q_chs)"
+    using \<open>?q_chs_s_after_q_chs \<noteq> []\<close> hd_map by blast
+  finally have "take block_for_q_chs_len (concat (map ?f ?q_chs_s_after_q_chs)) =
+                ?f (hd ?q_chs_s_after_q_chs)" by blast
+  with \<open>?blks_after_label = concat (map ?f ?q_chs_s_after_q_chs)\<close>
+       \<open>hd ?q_chs_s_after_q_chs = (q, chs)\<close>
+  have "take block_for_q_chs_len ?blks_after_label = ?f (q, chs)"
+    by argo
+
+  from entrance_block_length have entrance_length:
+    "length (HALT\<^sub>l # entrance_block) = Suc entrance_block_len"
+    by auto
+  then have "Suc entrance_block_len + block_for_q_chs_len * ?idx \<ge> length (HALT\<^sub>l # entrance_block)"
+    by linarith
+  then have "drop (Suc entrance_block_len + block_for_q_chs_len * ?idx) (HALT\<^sub>l # entrance_block) = []"
+    by fastforce
+  moreover
+  have "Suc entrance_block_len + block_for_q_chs_len * ?idx - length (HALT\<^sub>l # entrance_block) =
+        block_for_q_chs_len * ?idx"
+    using entrance_length by presburger
+  ultimately
+  have "drop (Suc entrance_block_len + block_for_q_chs_len * ?idx) GOTO_on_List_Prog =
+        drop (block_for_q_chs_len * index q_chs_enum_list (q, chs)) (blocks_for_actions @ [HALT\<^sub>l])"
+    using drop_append [where ?n = "Suc entrance_block_len + block_for_q_chs_len * ?idx"
+                         and ?xs = "HALT\<^sub>l # entrance_block"
+                         and ?ys = "blocks_for_actions @ [HALT\<^sub>l]"]
+    by (smt (verit, del_insts) Cons_eq_appendI self_append_conv2)
+  also have "... = ?blks_after_label @ [HALT\<^sub>l]"
+    using label_part_2_not_exceed_prog
+    using drop_append [where ?n = "block_for_q_chs_len * ?idx"
+                         and ?xs = ?blks_after_label and ?ys = "[HALT\<^sub>l]"]
+    by auto
+  finally have "drop (label_of_block_for_q_chs (q, chs)) GOTO_on_List_Prog = ?blks_after_label @ [HALT\<^sub>l]"
+    by (metis label_of_block_for_q_chs.simps)
+  moreover
+  have "take block_for_q_chs_len (?blks_after_label @ [HALT\<^sub>l]) =
+        take block_for_q_chs_len ?blks_after_label"
+    using take_append [where ?n = block_for_q_chs_len
+                         and ?xs = ?blks_after_label and ?ys = "[HALT\<^sub>l]"]
+    using \<open>length ?blks_after_label \<ge> block_for_q_chs_len\<close>
+    by (metis append_Nil2 diff_is_0_eq take0)
+  ultimately
+  have "take block_for_q_chs_len (drop (label_of_block_for_q_chs (q, chs)) GOTO_on_List_Prog) =
+        take block_for_q_chs_len ?blks_after_label"
+    by presburger
+  moreover
+  have "?f (q, chs) = block_for_q_chs ((M ! q) chs)"
+    by fast
+  ultimately
+  show ?thesis
+    using \<open>take block_for_q_chs_len ?blks_after_label = ?f (q, chs)\<close>
+    by argo
+qed
 
 subsection \<open>Correctness of the transform function\<close>
 
+lemma from_entrance_jumps_to_the_right_label:
+  assumes "q_chs \<in> set q_chs_enum_list"
+    shows "GOTO_on_List_Prog \<turnstile>\<^sub>l
+           (pc_start, s) \<rightarrow>\<^bsub>Suc (Suc (index q_chs_enum_list q_chs))\<^esub>
+           (label_of_block_for_q_chs q_chs, s)"
+  sorry
+
+lemma block_for_q_chs_correct:
+  assumes "exe M (q, tps) = (q', tps')"
+    shows "GOTO_on_List_Prog \<turnstile>\<^sub>l
+           (label_of_block_for_q_chs (q, read tps), config_to_state (q, tps))
+           \<rightarrow>\<^bsub>block_for_q_chs_len\<^esub>
+           (pc_start, config_to_state (q', tps'))"
+  sorry
+
+lemma TM_to_GOTO_on_List_correct_for_single_step:
+  assumes "exe M (q, tps) = (q', tps')"
+    shows "GOTO_on_List_Prog \<turnstile>\<^sub>l
+           (pc_start, config_to_state (q, tps))
+           \<rightarrow>\<^bsub>Suc (Suc (index q_chs_enum_list q_chs)) + block_for_q_chs_len\<^esub>
+           (pc_start, config_to_state (q', tps'))"
+  sorry
+
+lemma GOTO_on_List_correctly_ends:
+  "GOTO_on_List_Prog \<turnstile>\<^sub>l
+   (pc_start, config_to_state (Q, tps)) \<rightarrow>\<^bsub>1\<^esub> (pc_halt, config_to_state (Q, tps))"
+  sorry
+
 theorem TM_to_GOTO_on_List_correct:
-  assumes "GOTO_on_List_Prog \<turnstile>\<^sub>l (1, s\<^sub>0) \<rightarrow>* (0, s)"
+  assumes "GOTO_on_List_Prog \<turnstile>\<^sub>l (pc_start, s\<^sub>0) \<rightarrow>* (pc_halt, s)"
     shows "\<forall>k < K. \<forall>p < MAX_LEN. (s (TP k)) ! p = (TPS':::k) p"
   sorry
 
