IMPminus_TM/TM_GOTO/List_Extra.thy
@@ -1,0 +1,79 @@
+theory List_Extra
+  imports Main
+begin
+
+lemma length_concat_same_length:
+  "\<forall>xs \<in> set xss. length xs = len \<Longrightarrow> length (concat xss) = len * length xss"
+proof -
+  assume "\<forall>xs \<in> set xss. length xs = len"
+  then have "map length xss = replicate (length xss) len"
+    using map_replicate_const [where ?k = len and ?lst = xss]
+    by (metis map_eq_conv)
+  moreover
+  have "sum_list (replicate (length xss) len) = (length xss) * len"
+    by (simp add: sum_list_replicate)
+  ultimately
+  show "length (concat xss) = len * length xss"
+    by (simp add: length_concat)
+qed
+
+lemma drop_concat_same_length:
+  "\<forall>xs \<in> set xss. length xs = len \<Longrightarrow> drop (len * n) (concat xss) = concat (drop n xss)"
+proof (induction xss arbitrary: n)
+  case Nil
+  then show ?case by auto
+next
+  case (Cons xs xss)
+  then show ?case
+  proof (cases n)
+    case 0
+    then show ?thesis by auto
+  next
+    case (Suc m)
+    with \<open>\<forall>xs\<in>set (xs # xss). length xs = len\<close>
+    have "drop (len * (Suc m)) (concat (xs # xss)) = drop (len * m) (concat xss)"
+      by auto
+    moreover
+    have "concat (drop (Suc m) (xs # xss)) = concat (drop m xss)"
+      by simp
+    moreover
+    from Cons have "drop (len * m) (concat xss) = concat (drop m xss)"
+      by auto
+    ultimately
+    show ?thesis
+      using \<open>n = Suc m\<close> by presburger
+  qed
+qed
+
+lemma take_concat_same_length:
+  "\<forall>xs \<in> set xss. length xs = len \<Longrightarrow> take (len * n) (concat xss) = concat (take n xss)"
+proof (induction xss arbitrary: n)
+  case Nil
+  then show ?case by auto
+next
+  case (Cons xs xss)
+  then show ?case
+  proof (cases n)
+    case 0
+    then show ?thesis by auto
+  next
+    case (Suc m)
+    with \<open>\<forall>xs\<in>set (xs # xss). length xs = len\<close>
+    have "take (len * (Suc m)) (concat (xs # xss)) = xs @ take (len * m) (concat xss)"
+      by auto
+    moreover
+    have "concat (take (Suc m) (xs # xss)) = xs @ concat (take m xss)"
+      by simp
+    moreover
+    from Cons have "take (len * m) (concat xss) = concat (take m xss)"
+      by auto
+    ultimately
+    show ?thesis
+      using \<open>n = Suc m\<close> by presburger
+  qed
+qed
+
+lemma concat_take_1_is_hd: "xss \<noteq> [] \<Longrightarrow> concat (take 1 xss) = hd xss"
+  by (induction xss) auto
+
+end
